Construct the list the right way around in the first place rather than constructing it reversed and then reversing it again to ensure it ends up the right way around

convolutional_codesScript.sml
@@ -1955,22 +1955,29 @@ Definition vd_step_back_def:
 End
 
 (* -------------------------------------------------------------------------- *)
-(* Returns the optimal path going from back to front.                         *)
+(* Returns the optimal path leading to state s at timestep t, with respect to *)
+(* the bitstring bs that we are trying to approximate.                        *)
 (*                                                                            *)
 (* Returns the path as a list of all states encountered along the path,       *)
 (* including the very first and last states, with the first element of this   *)
-(* list being the last state encountered in the path, and the last element of *)
-(* this list being the first state encountered in the path.                   *)
+(* list being the first state encountered in the path, and the last element   *)
+(* of this list being the last state encountered in the path.                 *)
 (*                                                                            *)
 (* vd stands for Viterbi Decode                                               *)
 (* -------------------------------------------------------------------------- *)
 (* TODO: Repeatedly calling vd_step_back is slow, because it regenerates the  *)
 (* trellis at each step.                                                      *)
 (* -------------------------------------------------------------------------- *)
+Definition vd_find_optimal_path_def:
+  vd_find_optimal_path m bs s 0 = [s] ∧
+  vd_find_optimal_path m bs s (SUC t) =
+  SNOC s (vd_find_optimal_path m bs (vd_step_back m bs s (SUC t)) t)
+End
+
+(* -------------------------------------------------------------------------- *)
+(* Added for legacy reasons. Do not use in new code. Phase out where possible.*)(* -------------------------------------------------------------------------- *)
 Definition vd_find_optimal_reversed_path_def:
-  vd_find_optimal_reversed_path m bs s 0 = [s] ∧
-  vd_find_optimal_reversed_path m bs s (SUC t) =
-  s :: vd_find_optimal_reversed_path m bs (vd_step_back m bs s (SUC t)) t
+  vd_find_optimal_reversed_path m bs s t = REVERSE (vd_find_optimal_path m bs s t)
 End
 
 (* -------------------------------------------------------------------------- *)
@@ -2018,19 +2025,6 @@ Theorem vd_find_optimal_reversed_path_test:
 Proof
   EVAL_TAC
 QED
-
-(*
---------------------------------------------------------------------------
-*)
-(* See comment for vd_find_optimal_reversed_path                              *)
-(*                                                                            *)
-(* Reverses the path returned
- by that function to ensure the path is returned *)
-(* in the forwards direction                                                  *)
-(* -------------------------------------------------------------------------- *)
-Definition vd_find_optimal_path_def:
-  vd_find_optimal_path m bs s t = REVERSE (vd_find_optimal_reversed_path m bs s t)
-End
 
 (* -------------------------------------------------------------------------- *)
 (* An unknown, valid state, used for testing purposes                         *)
@@ -2553,44 +2547,23 @@ Proof
   >> gvs[best_origin_is_valid]   
 QED
 
-Theorem vd_find_optimal_reversed_path_length[simp]:
-  ∀m bs s t.
-  wfmachine m ∧
-  s < m.num_states ⇒
-  LENGTH (vd_find_optimal_reversed_path m bs s t) = t + 1
-Proof
-  (* Induct over t *)
-  gen_tac
-  >> Induct_on ‘t’ >> rpt strip_tac
-  >- EVAL_TAC
-  (* Expand out definitions *)
-  >> gvs[vd_find_optimal_reversed_path_def, vd_step_back_def]
-  (* Deal with the case where the previous state is NONE, so that we can work
-     on the more interesting case where there is a preivous state *)
-  >> qspecl_then [‘m’, ‘bs’, ‘SUC t’, ‘s’] assume_tac (cj 1 viterbi_trellis_row_prev_state_valid)
-  >> gvs[]
-  >> qmatch_asmsub_abbrev_tac ‘s' ≠ NONE’
-  >> Cases_on ‘s'’ >> gvs[]
-  (* Use the inductive hypothesis to finish the proof, leaving open the
-     unproven assumption that travelling back to a prior state resulted
-     om a valid state.*)
-  >> last_x_assum $ qspecl_then [‘bs’, ‘x’] assume_tac
-  >> gvs[]
-  >> ‘x < m.num_states’ suffices_by decide_tac
-  >> pop_assum kall_tac
-  (* We just need to prove that travelling back through the trellis
-        results in a valid state *)
-  >> qspecl_then [‘m’, ‘bs’, ‘(SUC t)’, ‘s’] assume_tac (cj 2 viterbi_trellis_row_prev_state_valid)
-  >> gvs[]
-QED
-
 Theorem vd_find_optimal_path_length[simp]:
   ∀m bs s t.
-  wfmachine m ∧
-  s < m.num_states ⇒
   LENGTH (vd_find_optimal_path m bs s t) = t + 1
 Proof
-  gvs[vd_find_optimal_path_def]
+  gen_tac
+  (* Induct over t *)
+  >> Induct_on ‘t’
+  >- (rpt strip_tac >> EVAL_TAC)
+  (* Expand out definitions *)
+  >> gvs[vd_find_optimal_path_def, vd_step_back_def]
+QED
+
+Theorem vd_find_optimal_reversed_path_length[simp]:
+  ∀m bs s t.
+  LENGTH (vd_find_optimal_reversed_path m bs s t) = t + 1
+Proof
+  gvs[vd_find_optimal_reversed_path_def]
 QED
 
 Theorem get_better_final_state_foldr_mem:
@@ -2615,21 +2588,6 @@ Theorem vd_find_optimal_reversed_path_time_zero[simp]:
   vd_find_optimal_reversed_path m bs s 0 = [s]
 Proof
   rpt strip_tac >> EVAL_TAC
-QED
-
-Theorem vd_find_optimal_reversed_path_length[simp]:
-  ∀m bs s t.
-  LENGTH (vd_find_optimal_reversed_path m bs s t) = t + 1
-Proof
-  Induct_on ‘t’ >> rpt strip_tac >> gvs[]
-  >> gvs[vd_find_optimal_reversed_path_def]
-QED
-
-Theorem vd_find_optimal_path_length[simp]:
-  ∀m bs s t.
-  LENGTH (vd_find_optimal_path m bs s t) = t + 1
-Proof
-  gvs[vd_find_optimal_path_def, vd_find_optimal_reversed_path_length]
 QED
 
 Theorem vd_find_optimal_code_length[simp]:
@@ -2702,9 +2660,8 @@ Theorem vd_find_optimal_path_nonempty[simp]:
   vd_find_optimal_path m bs s t ≠ []
 Proof
   rpt strip_tac
-  >> gvs[vd_find_optimal_path_def]
   >> Cases_on ‘t’
-  >> gvs[vd_find_optimal_reversed_path_def]
+  >> gvs[vd_find_optimal_path_def]
 QED
 
 Theorem vd_step_back_is_valid[simp]:
